Act on more PR review comments
Move files from src/SDK/MessageHeader/ to src/SDK/.
Rename constant ValidIDs to VALID_IDS.
Simplify return value of StringReader.ReadSeq.
Simplify logic of StringReader.Read.
Add a TODO to StringWriter.HasRemainingCapacity.
Add method Deserialize.DeserializeHeader, and export it in lieu of DeserializeHeaderBody and DeserializeHeaderAuthentication.
Moved DeserializeHeaderBody and DeserializeHeaderAuthentication closer to the top of file Deserialize.dfy (no change of those methods).
Inline and then remove ValidIVLength predicate.
Add `0 < |entries|` to EncryptedDataKeys.Valid().

src/SDK/AlgorithmSuite.dfy
@@ -10,9 +10,9 @@ module AlgorithmSuite {
   import C = Cipher
   import Digests
 
-  const ValidIDs: set<uint16> := {0x0378, 0x0346, 0x0214, 0x0178, 0x0146, 0x0114, 0x0078, 0x0046, 0x0014};
+  const VALID_IDS: set<uint16> := {0x0378, 0x0346, 0x0214, 0x0178, 0x0146, 0x0114, 0x0078, 0x0046, 0x0014};
 
-  newtype ID = x | x in ValidIDs witness 0x0014
+  newtype ID = x | x in VALID_IDS witness 0x0014
   {
     function method KeyLength(): nat {
       Suite[this].params.keyLen as nat
@@ -68,9 +68,9 @@ module AlgorithmSuite {
   }
 
   lemma ValidIDsAreSuiteKeys()
-    ensures ValidIDs == set id | id in Suite.Keys :: id as uint16
+    ensures VALID_IDS == set id | id in Suite.Keys :: id as uint16
   {
-    forall x | x in ValidIDs
+    forall x | x in VALID_IDS
       ensures exists id :: id in Suite.Keys && id as uint16 == x
     {
       assert x as ID in Suite.Keys;
